changed last_block to last_padded_block, fixed test file

specs/Spec.Blake2.fst
@@ -402,7 +402,8 @@ val blake2_update_last:
   -> s:state a ->
   Tot (state a)
 
-let get_last_block (a:alg) (m:bytes) (rem:nat{rem <= length m /\ rem <= size_block a}) : block_s a =
+let get_last_padded_block (a:alg) (m:bytes)
+    (rem:nat{rem <= length m /\ rem <= size_block a}) : block_s a =
   let last = Seq.slice m (length m - rem) (length m) in
   let last_block = create (size_block a) (u8 0) in
   let last_block = update_sub last_block 0 rem last in
@@ -411,7 +412,7 @@ let get_last_block (a:alg) (m:bytes) (rem:nat{rem <= length m /\ rem <= size_blo
 let blake2_update_last a prev rem m s =
   let inlen = length m in
   let totlen = prev + inlen in
-  let last_block = get_last_block a m rem in
+  let last_block = get_last_padded_block a m rem in
   blake2_update_block a true totlen last_block s
 
 val blake2_update_blocks:
@@ -421,7 +422,9 @@ val blake2_update_blocks:
   -> s:state a ->
   Tot (state a)
 
-let split (a:alg) (len:nat) : nb_rem:(nat & nat){let (nb,rem) = nb_rem in nb * size_block a + rem == len} =
+let split (a:alg) (len:nat)
+  : nb_rem:(nat & nat){let (nb,rem) = nb_rem in
+		   nb * size_block a + rem == len} =
   let nb = len / size_block a in
   let rem = len % size_block a in
   let nb' = if rem = 0 && nb > 0 then nb - 1 else nb in
